theory/x64_encode_cmovl_4.thy
@@ -1,0 +1,306 @@
+theory x64_encode_cmovl_4
+imports
+  Main
+  rBPFCommType
+  x64Syntax BitsOpMore
+begin
+
+
+lemma encode_cmovl_3_subgoal_1: "and 15 ((v::u8) >> 4) = 4 \<Longrightarrow> and 15 v \<noteq> 0 \<Longrightarrow>
+    \<not> bit v 3 \<Longrightarrow> \<not> bit v (Suc 0) \<Longrightarrow> bit v 2 \<Longrightarrow> bit v 0 \<Longrightarrow>
+    n < 8 \<Longrightarrow> bit v n \<Longrightarrow> bit (69::int) n"
+  apply (cases n, simp_all)
+  subgoal for n1 apply (cases n1, simp_all)
+    subgoal for n2 apply (cases n2, simp_all)
+      subgoal for n3 apply (cases n3, simp_all)
+        subgoal
+          by (simp add: bit_iff_odd_drop_bit even_iff_mod_2_eq_zero numeral_3_eq_3 one_and_eq) 
+        subgoal for n4 apply (cases n4, simp_all)
+          subgoal 
+            by (metis bit_1_0 bit_and_iff bit_numeral_Bit1_0 bit_word_iff_drop_bit_and eval_nat_numeral(2) not_bit_numeral_Bit0_0 numeral_3_eq_3 semiring_norm(26) semiring_norm(27))
+          subgoal for n5 apply (cases n5, simp_all)
+            subgoal for n6 apply (cases n6, simp_all)
+              done
+            done
+          done
+        done
+      done
+    done
+  done
+
+lemma encode_cmovl_3_subgoal_2: " and 15 ((v::u8) >> 4) = 4 \<Longrightarrow> and 15 v \<noteq> 0 \<Longrightarrow>
+     \<not> bit v 3 \<Longrightarrow> \<not> bit v (Suc 0) \<Longrightarrow> bit v 2 \<Longrightarrow> bit v 0 \<Longrightarrow> 
+    n < 8 \<Longrightarrow> bit (69::int) n \<Longrightarrow> bit v n"
+  apply (cases n, simp_all)
+  subgoal for n1 apply (cases n1, simp_all)
+    subgoal for n2 apply (cases n2, simp_all)
+      subgoal for n3 apply (cases n3, simp_all)
+        subgoal for n4 apply (cases n4, simp_all)
+          subgoal for n5 apply (cases n5, simp_all)
+            subgoal for n6 apply (cases n6, simp_all)
+              done
+            done
+          done
+        done
+      done
+    done
+  done
+
+lemma encode_cmovl_3_subgoal_3: "and 15 ((v::u8) >> 4) = 4 \<Longrightarrow> and 15 v \<noteq> 0 \<Longrightarrow>
+     \<not> bit v 3 \<Longrightarrow> \<not> bit v (Suc 0) \<Longrightarrow>
+    bit v 2 \<Longrightarrow> \<not> bit v 0 \<Longrightarrow> n < 8 \<Longrightarrow> bit v n \<Longrightarrow> bit (68::int) n"
+  apply (cases n, simp_all)
+  subgoal for n1 apply (cases n1, simp_all)
+    subgoal for n2 apply (cases n2, simp_all)
+      subgoal for n3 apply (cases n3, simp_all)
+        subgoal
+          by (simp add: bit_iff_odd_drop_bit even_iff_mod_2_eq_zero numeral_3_eq_3 one_and_eq) 
+        subgoal for n4 apply (cases n4, simp_all)
+          subgoal 
+            by (metis bit_1_0 bit_and_iff bit_numeral_Bit1_0 bit_word_iff_drop_bit_and eval_nat_numeral(2) not_bit_numeral_Bit0_0 numeral_3_eq_3 semiring_norm(26) semiring_norm(27))
+          subgoal for n5 apply (cases n5, simp_all)
+            subgoal for n6 apply (cases n6, simp_all)
+              done
+            done
+          done
+        done
+      done
+    done
+  done
+
+lemma encode_cmovl_3_subgoal_4: "and 15 ((v::u8) >> 4) = 4 \<Longrightarrow> and 15 v \<noteq> 0 \<Longrightarrow>
+    \<not> bit v 3 \<Longrightarrow> \<not> bit v (Suc 0) \<Longrightarrow>
+    bit v 2 \<Longrightarrow> \<not> bit v 0 \<Longrightarrow> n < 8 \<Longrightarrow> bit (68::int) n \<Longrightarrow> bit v n"
+  apply (cases n, simp_all)
+  subgoal for n1 apply (cases n1, simp_all)
+    subgoal for n2 apply (cases n2, simp_all)
+      subgoal for n3 apply (cases n3, simp_all)
+        subgoal for n4 apply (cases n4, simp_all)
+          subgoal for n5 apply (cases n5, simp_all)
+            subgoal for n6 apply (cases n6, simp_all)
+              done
+            done
+          done
+        done
+      done
+    done
+  done
+
+
+lemma encode_cmovl_3_subgoal_5 : " and 15 ((v::u8) >> 4) = 4 \<Longrightarrow> and 15 v \<noteq> 0 \<Longrightarrow>
+    \<not> bit v 3 \<Longrightarrow> \<not> bit v (Suc 0) \<Longrightarrow> \<not> bit v 2 \<Longrightarrow> bit v 0 \<Longrightarrow> 
+    n < 8 \<Longrightarrow> bit v n \<Longrightarrow> bit (65::int) n"
+  apply (cases n, simp_all)
+  subgoal for n1 apply (cases n1, simp_all)
+    subgoal for n2 apply (cases n2, simp_all)
+      subgoal
+        by (metis numeral_2_eq_2)
+      subgoal for n3 apply (cases n3, simp_all)
+        subgoal
+          by (metis numeral_3_eq_3)
+        subgoal for n4 apply (cases n4, simp_all)
+          subgoal
+            by (metis add_2_eq_Suc' bit_1_0 bit_and_iff bit_numeral_Bit1_0 bit_word_iff_drop_bit_and not_bit_numeral_Bit0_0 numeral_2_eq_2 numeral_Bit0)
+          subgoal for n5 apply (cases n5, simp_all)
+            subgoal for n6 apply (cases n6, simp_all)
+              done
+            done
+          done
+        done
+      done
+    done
+  done
+
+lemma encode_cmovl_3_subgoal_6: "and 15 ((v::u8) >> 4) = 4 \<Longrightarrow>
+    and 15 v \<noteq> 0 \<Longrightarrow> \<not> bit v 3 \<Longrightarrow> \<not> bit v (Suc 0) \<Longrightarrow> \<not> bit v 2 \<Longrightarrow> bit v 0 \<Longrightarrow>
+     n < 8 \<Longrightarrow> bit (65::int) n \<Longrightarrow> bit v n"
+  apply (cases n, simp_all)
+  subgoal for n1 apply (cases n1, simp_all)
+    subgoal for n2 apply (cases n2, simp_all)
+      subgoal for n3 apply (cases n3, simp_all)
+        subgoal for n4 apply (cases n4, simp_all)
+          subgoal for n5 apply (cases n5, simp_all)
+            subgoal for n6 apply (cases n6, simp_all)
+              done
+            done
+          done
+        done
+      done
+    done
+  done
+
+lemma encode_cmovl_3_subgoal_7: "
+    and 31 ((p::u8) >> 3) \<noteq> 25 \<Longrightarrow> and 15 (p >> 4) = 4 \<Longrightarrow> 
+    n < 8 \<Longrightarrow> bit p n \<Longrightarrow> \<not> bit (64::int) n \<Longrightarrow> bit (15::int) n"
+  apply (cases n, simp_all)
+  subgoal for n1 apply (cases n1, simp_all)
+    subgoal for n2 apply (cases n2, simp_all)
+      subgoal for n3 apply (cases n3, simp_all)
+        subgoal for n4 apply (cases n4, simp_all)
+          subgoal
+            by (metis add_2_eq_Suc' bit_1_0 bit_and_iff bit_numeral_Bit1_0 bit_word_iff_drop_bit_and not_bit_numeral_Bit0_0 numeral_2_eq_2 numeral_Bit0)
+          subgoal for n5 apply (cases n5, simp_all)
+            subgoal for n6 apply (cases n6, simp_all)
+              done
+            done
+          done
+        done
+      done
+    done
+  done
+
+lemma encode_cmovl_3_subgoal_8: "
+    and 31 ((p::u8) >> 3) \<noteq> 25 \<Longrightarrow> and 15 (p >> 4) = 4 \<Longrightarrow> n < 8 \<Longrightarrow> bit (64::int) n \<Longrightarrow> bit p n"
+  apply (cases n, simp_all)
+  subgoal for n1 apply (cases n1, simp_all) 
+    subgoal for n2 apply (cases n2, simp_all)
+      subgoal for n3 apply (cases n3, simp_all)
+        subgoal for n4 apply (cases n4, simp_all)
+          subgoal for n5 apply (cases n5, simp_all)
+            subgoal for n6 apply (cases n6, simp_all)
+              done
+            done
+          done
+        done
+      done
+    done
+  done
+
+lemma encode_cmovl_3_subgoal_9: "
+    and 3 ((k::u8) >> 6) = 3 \<Longrightarrow>
+    n < 8 \<Longrightarrow> \<not> bit (192::int) n \<Longrightarrow> bit (7::int) n \<Longrightarrow> \<not> bit (56::int) n \<Longrightarrow> 
+    bit (8::int) n \<Longrightarrow> 3 \<le> n \<Longrightarrow> bit v (n - 3) \<Longrightarrow> bit k n"
+  apply (cases n, simp_all)
+  subgoal for n1 apply (cases n1, simp_all) 
+    subgoal for n2 apply (cases n2, simp_all)
+        done
+      done
+    done
+
+lemma encode_cmovl_3_subgoal_k : "and 15 (v >> 4) = 4 \<Longrightarrow> and 15 v \<noteq> 0 \<Longrightarrow>
+    and 31 (p >> 3) \<noteq> 25 \<Longrightarrow>  and 15 (p >> 4) = 4 \<Longrightarrow> and 3 (k >> 6) = 3 \<Longrightarrow>
+    u8_of_cond test = and 15 p \<Longrightarrow>
+    u8_of_ireg dst = or (and 8 ((v >> 2) << 3)) (and 7 (k >> 3)) \<Longrightarrow>
+    u8_of_ireg src = or (and 8 (v << 3)) (and 7 k) \<Longrightarrow>
+    \<not> bit v 3 \<Longrightarrow> \<not> bit v (Suc 0) \<Longrightarrow>
+    or 64
+     (and (and (or (and 4 ((case bit (v >> 2) 0 of True \<Rightarrow> 1 | False \<Rightarrow> 0) << 2))
+                 (and (and (case bit v 0 of True \<Rightarrow> 1 | False \<Rightarrow> 0) (- 3)) (- 5)))
+            (- 9))
+       (- 241)) \<noteq> 64 \<Longrightarrow>
+    v =
+    or 64 (and (and (or (and 4 ((case bit (v >> 2) 0 of True \<Rightarrow> 1 | False \<Rightarrow> 0) << 2))
+                 (and (and (case bit v 0 of True \<Rightarrow> 1 | False \<Rightarrow> 0) (- 3)) (- 5)))
+            (- 9))
+       (- 241)) \<and>
+    p = or (and 15 p) 64 \<and>
+    k =
+    or 192
+     (and (or (and 56 (or (and 64 ((v >> 2) << 6)) (and 56 ((k >> 3) << 3))))
+            (and (and 7 (or (and 8 (v << 3)) (and 7 k))) (- 57)))
+       (- 193))"
+  apply (rule conjI)
+  subgoal
+    apply (cases "bit (v >> 2) 0"; cases "bit v 0", simp_all)
+    subgoal
+      apply (rule bit_eqI)
+      subgoal for n
+        apply (auto simp add: bit_simps)
+        subgoal using encode_cmovl_3_subgoal_1 by blast
+        subgoal using encode_cmovl_3_subgoal_2 by blast
+          done
+        done
+    subgoal
+      apply (rule bit_eqI)
+      subgoal for n
+        apply (auto simp add: bit_simps)
+        subgoal using encode_cmovl_3_subgoal_3 by blast
+        subgoal using encode_cmovl_3_subgoal_4 by blast
+          done
+        done
+      subgoal
+      apply (rule bit_eqI)
+      subgoal for n
+        apply (auto simp add: bit_simps)
+        subgoal using encode_cmovl_3_subgoal_5 by blast
+        subgoal using encode_cmovl_3_subgoal_6 by blast
+          done
+        done
+      done
+
+    subgoal
+      apply (rule conjI)
+       apply (cases "bit (v >> 2) 0"; cases "bit v 0", simp_all)
+      subgoal
+        apply (rule bit_eqI)
+        subgoal for n
+          apply (auto simp add: bit_simps)
+          subgoal using encode_cmovl_3_subgoal_7 by blast
+          subgoal using encode_cmovl_3_subgoal_8 by blast
+          done
+        done
+      subgoal
+        apply (rule bit_eqI)
+        subgoal for n
+          apply (auto simp add: bit_simps)
+          subgoal using encode_cmovl_3_subgoal_7 by blast
+          subgoal using encode_cmovl_3_subgoal_8 by blast
+          done
+        done
+      subgoal
+        apply (rule bit_eqI)
+        subgoal for n
+          apply (auto simp add: bit_simps)
+          subgoal using encode_cmovl_3_subgoal_7 by blast
+          subgoal using encode_cmovl_3_subgoal_8 by blast
+          done
+        done
+
+      apply (rule bit_eqI)
+      apply (cases "bit (v >> 2) 0"; cases "bit v 0", simp_all)
+      subgoal for n
+        apply (auto simp add: bit_simps)
+        subgoal using encode_cmovl_3_subgoal_9 by blast
+        done
+      subgoal for n
+        apply (auto simp add: bit_simps)
+        subgoal using encode_cmovl_3_subgoal_9 by blast
+        done
+      subgoal for n
+        apply (auto simp add: bit_simps)
+        subgoal using encode_cmovl_3_subgoal_9 by blast
+        done
+      done
+    done
+
+
+lemma encode_cmovl_3: "
+    and 15 (v >> 4) = 4 \<Longrightarrow> and 15 v \<noteq> 0 \<Longrightarrow>
+    and 31 (p >> 3) \<noteq> 25 \<Longrightarrow> and 15 (p >> 4) = 4 \<Longrightarrow>         
+    and 3 (k >> 6) = 3 \<Longrightarrow>
+    cond_of_u8 (and 15 p) = Some test \<Longrightarrow>
+    ireg_of_u8 (bitfield_insert_u8 3 (Suc 0) (and 7 (k >> 3)) (and 1 (v >> 2))) =  Some dst \<Longrightarrow>
+    ireg_of_u8 (bitfield_insert_u8 3 (Suc 0) (and 7 k) (and 1 v)) = Some src \<Longrightarrow>
+    \<not> bit v 3 \<Longrightarrow> \<not> bit v (Suc 0) \<Longrightarrow>
+    bitfield_insert_u8 4 4
+     (bitfield_insert_u8 3 (Suc 0)
+       (bitfield_insert_u8 2 (Suc 0)
+         (bitfield_insert_u8 (Suc 0) (Suc 0) (u8_of_bool (and (u8_of_ireg src) 8 \<noteq> 0)) 0)
+         (u8_of_bool (and (u8_of_ireg dst) 8 \<noteq> 0)))
+       0) 4 \<noteq> 64 \<Longrightarrow>
+    v =
+    bitfield_insert_u8 4 4
+     (bitfield_insert_u8 3 (Suc 0)
+       (bitfield_insert_u8 2 (Suc 0)
+         (bitfield_insert_u8 (Suc 0) (Suc 0) (u8_of_bool (and (u8_of_ireg src) 8 \<noteq> 0)) 0)
+         (u8_of_bool (and (u8_of_ireg dst) 8 \<noteq> 0)))
+       0) 4 \<and>
+    p = bitfield_insert_u8 0 4 64 (u8_of_cond test) \<and>
+    k = bitfield_insert_u8 6 2 (bitfield_insert_u8 3 3 (and 7 (u8_of_ireg src)) (and 7 (u8_of_ireg dst))) 3"
+  apply (simp add: u8_of_ireg_of_u8_iff[symmetric] and_1_eq_1)
+  apply (simp add: u8_of_cond_of_u8_iff[symmetric])
+  apply (unfold bitfield_insert_u8_def u8_of_bool_def Let_def)
+  apply simp
+  using encode_cmovl_3_subgoal_k by blast
+
+end
