theory/x64_encode_movl_rr_3.thy
@@ -5,20 +5,36 @@ imports
   x64Syntax BitsOpMore
 begin
 
-lemma encode_movl_rr_3: " and 15 (v >> 4) = 4 \<Longrightarrow> and 15 (v) \<noteq> 0 \<Longrightarrow>and 3 (k >> 6) = 3 \<Longrightarrow>
+lemma encode_movl_rr_3_subgoal_1:"
+  \<not>bit v 3 \<Longrightarrow> \<not>bit v (Suc 0) \<Longrightarrow> \<not> bit (v >> 2) 0 \<Longrightarrow> \<not> bit v 0 \<Longrightarrow> and 15 (v::u8) = 0 
+"
+  apply (rule bit_eqI)
+  apply (auto simp add: bit_simps)
+  subgoal for n1 apply (cases n1, simp_all)
+    subgoal for n2 apply (cases n2, simp_all)
+      subgoal for n3 apply (cases n3, simp_all)
+        apply (metis numeral_2_eq_2)
+        subgoal for n4 apply (cases n4, simp_all)
+          by (metis numeral_3_eq_3)
+        done
+      done
+    done
+  done
+
+lemma encode_movl_rr_3: "
+    and 15 (v >> 4) = 4 \<Longrightarrow> and 15 v \<noteq> 0 \<Longrightarrow> and 3 (k >> 6) = 3 \<Longrightarrow>
     ireg_of_u8 (bitfield_insert_u8 3 (Suc 0) (and 7 (k >> 3)) (and 1 (v >> 2))) = Some src \<Longrightarrow>
     ireg_of_u8 (bitfield_insert_u8 3 (Suc 0) (and 7 k) (and 1 v)) = Some dst \<Longrightarrow>
-    \<not> bit v 3 \<Longrightarrow> \<not> bit v (Suc 0) \<Longrightarrow>bit v 2 \<Longrightarrow>
+    \<not> bit v 3 \<Longrightarrow> \<not> bit v (Suc 0) \<Longrightarrow>
     bitfield_insert_u8 4 4
      (bitfield_insert_u8 3 (Suc 0)
        (bitfield_insert_u8 2 (Suc 0) (bitfield_insert_u8 (Suc 0) (Suc 0) (u8_of_bool (and (u8_of_ireg dst) 8 \<noteq> 0)) 0)
          (u8_of_bool (and (u8_of_ireg src) 8 \<noteq> 0)))
        0)
-     4 =
-    64  \<Longrightarrow> False"
+     4 = 64 \<Longrightarrow>False"
   apply (simp add: u8_of_ireg_of_u8_iff[symmetric])
   apply (simp add: bitfield_insert_u8_def Let_def u8_of_bool_def and_1_eq_1)
-  apply (cases "and (u8_of_ireg dst) 8 \<noteq> 0", simp_all)
-  done
+  apply (cases "bit (v >> 2) 0"; cases "bit v 0", simp_all)
+  using encode_movl_rr_3_subgoal_1 by blast
 
 end
