theory/x64_encode_movl_rr_4.thy
@@ -45,18 +45,20 @@ lemma encode_movl_rr_4_subgoal_2: "and 15 ((v::u8) >> 4) = 4 \<Longrightarrow> a
     done
   done
 
-lemma encode_movl_rr_4_subgoal_3: "and 15 ((v::u8) >> 4) = 4 \<Longrightarrow> and 3 ((k::u8) >> 6) = 3 \<Longrightarrow>
-  \<not> bit v 3 \<Longrightarrow> \<not> bit v (Suc 0) \<Longrightarrow> bit v 2 \<Longrightarrow>
-  \<not> bit v 0 \<Longrightarrow> n < 8 \<Longrightarrow> bit v n \<Longrightarrow> bit (68::int) n"
+
+lemma encode_movl_rr_4_subgoal_3 : "and 15 ((v::u8) >> 4) = 4 \<Longrightarrow> and 15 v \<noteq> 0 \<Longrightarrow>
+  \<not> bit v 3 \<Longrightarrow> \<not> bit v (Suc 0) \<Longrightarrow> bit v 0 \<Longrightarrow> \<not> bit v 2 \<Longrightarrow> n < 8 \<Longrightarrow> bit v n \<Longrightarrow> bit (65::u8) n"
   apply (cases n, simp_all)
   subgoal for n1 apply (cases n1, simp_all)
     subgoal for n2 apply (cases n2, simp_all)
+      subgoal
+        by (metis numeral_2_eq_2) 
       subgoal for n3 apply (cases n3, simp_all)
         subgoal
-          by (simp add: bit_iff_odd_drop_bit even_iff_mod_2_eq_zero numeral_3_eq_3 one_and_eq) 
+          by (metis numeral_3_eq_3)
         subgoal for n4 apply (cases n4, simp_all)
           subgoal
-            by (metis bit_1_0 bit_and_iff bit_numeral_Bit1_0 bit_word_iff_drop_bit_and eval_nat_numeral(2) not_bit_numeral_Bit0_0 numeral_3_eq_3 semiring_norm(26) semiring_norm(27))
+            by (metis add_2_eq_Suc' bit_1_0 bit_and_iff bit_numeral_Bit1_0 bit_word_iff_drop_bit_and not_bit_numeral_Bit0_0 numeral_2_eq_2 numeral_Bit0)
           subgoal for n5 apply (cases n5, simp_all)
             subgoal for n6 apply (cases n6, simp_all)
               done
@@ -67,9 +69,9 @@ lemma encode_movl_rr_4_subgoal_3: "and 15 ((v::u8) >> 4) = 4 \<Longrightarrow> a
     done
   done
 
-lemma encode_movl_rr_4_subgoal_4 : "and 15 ((v::u8) >> 4) = 4 \<Longrightarrow> and 3 ((k::u8) >> 6) = 3 \<Longrightarrow>
-  \<not> bit v 3 \<Longrightarrow> \<not> bit v (Suc 0) \<Longrightarrow> bit v 2 \<Longrightarrow>
-  \<not> bit v 0 \<Longrightarrow> n < 8 \<Longrightarrow> bit (68::int) n \<Longrightarrow> bit v n"
+
+lemma encode_movl_rr_4_subgoal_4: "and 15 ((v::u8) >> 4) = 4 \<Longrightarrow> and 15 v \<noteq> 0 \<Longrightarrow>
+     \<not> bit v 3 \<Longrightarrow> \<not> bit v (Suc 0) \<Longrightarrow> bit v 0 \<Longrightarrow> \<not> bit v 2 \<Longrightarrow> n < 8 \<Longrightarrow> bit (65::u8) n \<Longrightarrow> bit v n"
   apply (cases n, simp_all)
   subgoal for n1 apply (cases n1, simp_all)
     subgoal for n2 apply (cases n2, simp_all)
@@ -85,20 +87,69 @@ lemma encode_movl_rr_4_subgoal_4 : "and 15 ((v::u8) >> 4) = 4 \<Longrightarrow> 
     done
   done
 
-lemma encode_movl_rr_4_subgoal_k : "and 15 (v >> 4) = 4 \<Longrightarrow>
-    and 15 v \<noteq> 0 \<Longrightarrow>
-    and 3 (k >> 6) = 3 \<Longrightarrow>
-    u8_of_ireg src = or 8 (and 7 (k >> 3)) \<Longrightarrow>
+lemma encode_movl_rr_4_subgoal_5 : "and 15 ((v::u8) >> 4) = 4 \<Longrightarrow> and 15 v \<noteq> 0 \<Longrightarrow>
+  \<not> bit v 3 \<Longrightarrow> \<not> bit v (Suc 0) \<Longrightarrow> \<not> bit v 0 \<Longrightarrow> bit v 2 \<Longrightarrow> n < 8 \<Longrightarrow> bit v n \<Longrightarrow> bit (68::u8) n"
+  apply (cases n, simp_all)
+  subgoal for n1 apply (cases n1, simp_all)
+    subgoal for n2 apply (cases n2, simp_all)
+      subgoal for n3 apply (cases n3, simp_all)
+      subgoal
+        by (metis numeral_3_eq_3) 
+      subgoal for n4 apply (cases n4, simp_all)
+          subgoal
+            by (metis add_2_eq_Suc' bit_1_0 bit_and_iff bit_numeral_Bit1_0 bit_word_iff_drop_bit_and not_bit_numeral_Bit0_0 numeral_2_eq_2 numeral_Bit0)
+          subgoal for n5 apply (cases n5, simp_all)
+            subgoal for n6 apply (cases n6, simp_all)
+              done
+            done
+          done
+        done
+      done
+    done
+  done
+
+
+lemma encode_movl_rr_4_subgoal_6: "and 15 ((v::u8) >> 4) = 4 \<Longrightarrow> and 15 v \<noteq> 0 \<Longrightarrow>
+     \<not> bit v 3 \<Longrightarrow> \<not> bit v (Suc 0) \<Longrightarrow> \<not> bit v 0 \<Longrightarrow> bit v 2 \<Longrightarrow> n < 8 \<Longrightarrow> bit (68::u8) n \<Longrightarrow> bit v n"
+  apply (cases n, simp_all)
+  subgoal for n1 apply (cases n1, simp_all)
+    subgoal for n2 apply (cases n2, simp_all)
+      subgoal for n3 apply (cases n3, simp_all)
+        subgoal for n4 apply (cases n4, simp_all)
+          subgoal for n5 apply (cases n5, simp_all)
+            subgoal for n6 apply (cases n6, simp_all)
+              done
+            done
+          done
+        done
+      done
+    done
+  done
+
+
+
+lemma encode_movl_rr_4_subgoal_k : "and 15 (v >> 4) = 4 \<Longrightarrow> and 15 v \<noteq> 0 \<Longrightarrow> and 3 (k >> 6) = 3 \<Longrightarrow>
+    u8_of_ireg src = or (and 8 ((v >> 2) << 3)) (and 7 (k >> 3)) \<Longrightarrow>
     u8_of_ireg dst = or (and 8 (v << 3)) (and 7 k) \<Longrightarrow>
-    \<not> bit v 3 \<Longrightarrow>
-    \<not> bit v (Suc 0) \<Longrightarrow>
-    bit v 2 \<Longrightarrow>
-    or 64 (and (and (or 4 (and (and (case bit v 0 of True \<Rightarrow> 1 | False \<Rightarrow> 0) (- 3)) (- 5))) (- 9)) (- 241)) \<noteq> 64 \<Longrightarrow>
-    v = or 64 (and (and (or 4 (and (and (case bit v 0 of True \<Rightarrow> 1 | False \<Rightarrow> 0) (- 3)) (- 5))) (- 9)) (- 241)) \<and>
-    k = or 192 (and (or (and 56 (or 64 (and 56 ((k >> 3) << 3)))) (and (and 7 (or (and 8 (v << 3)) (and 7 k))) (- 57))) (- 193))"
+    \<not> bit v 3 \<Longrightarrow> \<not> bit v (Suc 0) \<Longrightarrow>
+    or 64
+     (and (and (or (and 4 ((case bit (v >> 2) 0 of True \<Rightarrow> 1 | False \<Rightarrow> 0) << 2))
+                 (and (and (case bit v 0 of True \<Rightarrow> 1 | False \<Rightarrow> 0) (- 3)) (- 5)))
+            (- 9))
+       (- 241)) \<noteq>
+    64 \<Longrightarrow>
+    v =
+    or 64
+     (and (and (or (and 4 ((case bit (v >> 2) 0 of True \<Rightarrow> 1 | False \<Rightarrow> 0) << 2))
+                 (and (and (case bit v 0 of True \<Rightarrow> 1 | False \<Rightarrow> 0) (- 3)) (- 5)))
+            (- 9))
+       (- 241)) \<and>
+    k =
+    or 192 (and (or (and 56 (or (and 64 ((v >> 2) << 6)) (and 56 ((k >> 3) << 3)))) 
+    (and (and 7 (or (and 8 (v << 3)) (and 7 k))) (- 57))) (- 193))"
   apply (rule conjI)
   subgoal
-    apply (cases "bit v 0", simp_all)
+    apply (cases "bit v 0";cases "bit (v >> 2) 0 ", simp_all)
     subgoal
       apply (rule bit_eqI)
       subgoal for n
@@ -110,15 +161,33 @@ lemma encode_movl_rr_4_subgoal_k : "and 15 (v >> 4) = 4 \<Longrightarrow>
     subgoal
       apply (rule bit_eqI)
       subgoal for n
-        apply (auto simp add: bit_simps)
-        subgoal using encode_movl_rr_4_subgoal_3 by blast
-        subgoal using encode_movl_rr_4_subgoal_4 by blast
+        apply (auto simp add: bit_simps)  
+        subgoal using encode_movl_rr_4_subgoal_3 by simp
+        subgoal using encode_movl_rr_4_subgoal_4 by simp
+        done
+      done
+
+    subgoal
+      apply (rule bit_eqI)
+      subgoal for n
+        apply (auto simp add: bit_simps)  
+        subgoal using encode_movl_rr_4_subgoal_5 by simp
+        subgoal using encode_movl_rr_4_subgoal_6 by simp
         done
       done
     done
 
   subgoal
-    apply (cases "bit v 0", simp_all)
+    apply (cases "bit v 0";cases "bit (v >> 2) 0 ", simp_all)
+    subgoal
+      apply (rule bit_eqI)
+      subgoal for n
+        apply (simp add: bit_or_iff)
+        apply (auto simp add: bit_simps)
+        subgoal
+          using encode_movl_rr_1_subgoal_4 by blast
+        done
+      done
     subgoal
       apply (rule bit_eqI)
       subgoal for n
@@ -140,27 +209,26 @@ lemma encode_movl_rr_4_subgoal_k : "and 15 (v >> 4) = 4 \<Longrightarrow>
     done
   done
 
-
 lemma encode_movl_rr_4: "
     and 15 (v >> 4) = 4 \<Longrightarrow> and 15 v \<noteq> 0 \<Longrightarrow> and 3 (k >> 6) = 3 \<Longrightarrow>
     ireg_of_u8 (bitfield_insert_u8 3 (Suc 0) (and 7 (k >> 3)) (and 1 (v >> 2))) = Some src \<Longrightarrow>
-    ireg_of_u8 (bitfield_insert_u8 3 (Suc 0) (and 7 (k)) (and 1 v)) = Some dst \<Longrightarrow>
-    \<not> bit v 3 \<Longrightarrow> \<not> bit v (Suc 0) \<Longrightarrow> bit v 2 \<Longrightarrow> 
+    ireg_of_u8 (bitfield_insert_u8 3 (Suc 0) (and 7 k) (and 1 v)) = Some dst \<Longrightarrow>
+    \<not> bit v 3 \<Longrightarrow> \<not> bit v (Suc 0) \<Longrightarrow>
     bitfield_insert_u8 4 4
      (bitfield_insert_u8 3 (Suc 0)
        (bitfield_insert_u8 2 (Suc 0) (bitfield_insert_u8 (Suc 0) (Suc 0) (u8_of_bool (and (u8_of_ireg dst) 8 \<noteq> 0)) 0)
          (u8_of_bool (and (u8_of_ireg src) 8 \<noteq> 0)))
-       0) 4 \<noteq>  64 \<Longrightarrow>
-    v =  bitfield_insert_u8 4 4
-           (bitfield_insert_u8 3 (Suc 0)
-             (bitfield_insert_u8 2 (Suc 0) (bitfield_insert_u8 (Suc 0) (Suc 0) (u8_of_bool (and (u8_of_ireg dst) 8 \<noteq> 0)) 0)
-               (u8_of_bool (and (u8_of_ireg src) 8 \<noteq> 0)))
-             0) 4 \<and>
+       0) 4 \<noteq> 64 \<Longrightarrow>
+    v =
+    bitfield_insert_u8 4 4
+     (bitfield_insert_u8 3 (Suc 0)
+       (bitfield_insert_u8 2 (Suc 0) (bitfield_insert_u8 (Suc 0) (Suc 0) (u8_of_bool (and (u8_of_ireg dst) 8 \<noteq> 0)) 0)
+         (u8_of_bool (and (u8_of_ireg src) 8 \<noteq> 0)))
+       0) 4 \<and>
     k = bitfield_insert_u8 6 2 (bitfield_insert_u8 3 3 (and 7 (u8_of_ireg dst)) (and 7 (u8_of_ireg src))) 3"
   apply (simp add: u8_of_ireg_of_u8_iff[symmetric])
   apply (unfold bitfield_insert_u8_def u8_of_bool_def Let_def)
   apply simp
   using encode_movl_rr_4_subgoal_k by blast
-
 
 end
