theory/x64_encode_negl_r_1.thy
@@ -1,0 +1,83 @@
+theory x64_encode_negl_r_1
+imports
+  Main
+  rBPFCommType
+  x64Syntax BitsOpMore
+begin
+
+
+lemma encode_negl_r_1_subgoal_1: " and 7 ((v::u8) >> 3) = 3 \<Longrightarrow> bit v (Suc (Suc (Suc (Suc (Suc 0))))) \<Longrightarrow> False
+ "
+  apply (simp add: bit_eq_iff Suc3_eq_add_3)
+  apply (auto simp add: bit_simps)
+  apply (drule_tac x="2" in spec) by simp
+
+
+lemma encode_negl_r_1_subgoal_2: " and 7 ((v::u8) >> 3) = 3 \<Longrightarrow> bit v (Suc (Suc (Suc (Suc 0)))) "
+  apply (simp add: bit_eq_iff Suc3_eq_add_3 )
+  apply (auto simp add: bit_simps)
+  apply (drule_tac x="1" in spec) by simp
+
+
+lemma encode_negl_r_1: "
+    and 3 ((v::u8) >> 6) = 3 \<Longrightarrow>
+    and 7 (v >> 3) = 3 \<Longrightarrow>
+    ireg_of_u8 (bitfield_insert_u8 3 (Suc 0) (and 7 v) 0) = Some dst \<Longrightarrow>
+    bitfield_insert_u8 4 4
+     (bitfield_insert_u8 3 (Suc 0) 
+       (bitfield_insert_u8 2 (Suc 0) 
+         (bitfield_insert_u8 (Suc 0) (Suc 0) (u8_of_bool (and (u8_of_ireg dst) 8 \<noteq> 0)) 0) 0) 0) 4 = 64 \<Longrightarrow>
+     v = bitfield_insert_u8 6 2 (bitfield_insert_u8 3 3 (and 7 (u8_of_ireg dst)) 3) 3"
+  apply (simp add: u8_of_ireg_of_u8_iff[symmetric])
+  apply (unfold bitfield_insert_u8_def u8_of_bool_def Let_def)
+  apply simp
+  apply (rule bit_eqI)
+  apply (auto simp add: bit_simps)
+
+  subgoal for n1 apply (cases n1, simp_all)
+    subgoal for n2 apply (cases n2, simp_all)
+      subgoal for n3 apply (cases n3, simp_all)
+        subgoal for n4 apply (cases n4, simp_all)
+          subgoal for n5 apply (cases n5, simp_all)
+            subgoal for n6 apply (cases n6, simp_all)
+              subgoal 
+                using encode_negl_r_1_subgoal_1 by blast
+              subgoal for n7 apply (cases n7, simp_all)
+                done
+              done
+            done
+          done
+        done
+      done
+    done
+
+  subgoal for n1 apply (cases n1, simp_all)
+    subgoal for n2 apply (cases n2, simp_all)
+      subgoal for n3 apply (cases n3, simp_all)
+        subgoal for n4 apply (cases n4, simp_all)
+          subgoal for n5 apply (cases n5, simp_all)
+            subgoal for n6 apply (cases n6, simp_all)
+              subgoal
+                using encode_negl_r_1_subgoal_1 by blast 
+                done
+              done
+            done
+          done
+        done
+      done
+ 
+  subgoal for n1 apply (cases n1, simp_all)
+    subgoal for n2 apply (cases n2, simp_all)
+      subgoal for n3 apply (cases n3, simp_all)
+        subgoal for n4 apply (cases n4, simp_all)
+          subgoal
+            by (metis bit_0 bit_and_iff bit_iff_odd_drop_bit bit_numeral_Bit1_0 numeral_3_eq_3)
+          subgoal for n5 apply (cases n5, simp_all)
+                using encode_negl_r_1_subgoal_2 by blast
+              done
+            done
+          done
+        done
+      done
+
+end
