theory/x64_encode_negl_r_2.thy
@@ -1,0 +1,21 @@
+theory x64_encode_negl_r_2
+imports
+  Main
+  rBPFCommType
+  x64Syntax BitsOpMore
+begin
+
+lemma encode_negl_r_2: "
+    and 3 (v >> 6) = 3 \<Longrightarrow> and 7 (v >> 3) = 3 \<Longrightarrow>
+    ireg_of_u8 (bitfield_insert_u8 3 (Suc 0) (and 7 v) 0) = Some dst \<Longrightarrow>
+    bitfield_insert_u8 4 4
+     (bitfield_insert_u8 3 (Suc 0)
+       (bitfield_insert_u8 2 (Suc 0) (bitfield_insert_u8 (Suc 0) (Suc 0) (u8_of_bool (and (u8_of_ireg dst) 8 \<noteq> 0)) 0) 0) 0)
+     4 \<noteq>
+    64  \<Longrightarrow> False"
+  apply (simp add: u8_of_ireg_of_u8_iff[symmetric])
+  apply (unfold bitfield_insert_u8_def u8_of_bool_def Let_def)
+  apply simp
+  done
+
+end
