theory/x64_encode_negl_r_3.thy
@@ -1,0 +1,43 @@
+theory x64_encode_negl_r_3
+imports
+  Main
+  rBPFCommType
+  x64Syntax BitsOpMore
+begin
+
+lemma encode_negl_3_subgoal_1 : "\<not> bit (v::u8) 3 \<Longrightarrow> \<not> bit v (Suc 0) \<Longrightarrow> \<not> bit (v >> 2) 0 \<Longrightarrow> \<not> bit v 0
+                                   \<Longrightarrow>  and 15 v = 0"
+  apply (rule bit_eqI)
+  apply (simp add: bit_simps)
+  subgoal for n
+  apply (cases n, simp_all)
+  subgoal for n1 apply (cases n1, simp_all)
+    subgoal for n2 apply (cases n2, simp_all)
+      subgoal
+        using numeral_2_eq_2 by argo 
+          subgoal for n3 apply (cases n3, simp_all)
+            using numeral_3_eq_3 by argo
+              done
+            done
+          done
+        done
+
+
+lemma encode_negl_r_3: "
+    and 15 (v >> 4) = 4 \<Longrightarrow> and 15 v \<noteq> 0 \<Longrightarrow>
+    and 3 (k >> 6) = 3 \<Longrightarrow> and 7 (k >> 3) = 3 \<Longrightarrow>
+    ireg_of_u8 (bitfield_insert_u8 3 (Suc 0) (and 7 k) (and 1 v)) = Some dst \<Longrightarrow>
+    \<not> bit v 3 \<Longrightarrow> \<not> bit v 2 \<Longrightarrow>
+    \<not> bit v (Suc 0) \<Longrightarrow>
+    bitfield_insert_u8 4 4
+     (bitfield_insert_u8 3 (Suc 0)
+       (bitfield_insert_u8 2 (Suc 0) (bitfield_insert_u8 (Suc 0) (Suc 0) (u8_of_bool (and (u8_of_ireg dst) 8 \<noteq> 0)) 0) 0) 0)
+     4 = 64  \<Longrightarrow> False"
+  apply (simp add: u8_of_ireg_of_u8_iff[symmetric])
+  apply (unfold bitfield_insert_u8_def u8_of_bool_def Let_def)
+  apply simp
+  apply (cases "bit v 0 ", simp_all)
+  using encode_negl_3_subgoal_1
+  by (meson bit_0 bit_iff_odd_drop_bit)
+
+end
