theory/x64_encode_negl_r_4.thy
@@ -1,0 +1,252 @@
+theory x64_encode_negl_r_4
+imports
+  Main
+  rBPFCommType
+  x64Syntax BitsOpMore
+begin
+
+
+lemma encode_negl_r_4_subgoal_1: "and 15 ((v::u8) >> 4) = 4 \<Longrightarrow> and 15 v \<noteq> 0 \<Longrightarrow>
+    \<not> bit v 3 \<Longrightarrow>  \<not> bit v 2 \<Longrightarrow>
+    \<not> bit v (Suc 0)  \<Longrightarrow> bit v 0 \<Longrightarrow> n < 8 \<Longrightarrow> bit v n \<Longrightarrow> bit (65::u8) n"
+  apply (cases n, simp_all)
+  subgoal for n1 apply (cases n1, simp_all)
+    subgoal for n2 apply (cases n2, simp_all)
+      apply (metis numeral_2_eq_2)
+      subgoal for n3 apply (cases n3, simp_all)
+        subgoal
+          by (simp add: numeral_3_eq_3)
+        subgoal for n4 apply (cases n4, simp_all)
+          subgoal
+            by (metis add_2_eq_Suc' bit_1_0 bit_and_iff bit_numeral_Bit1_0 bit_word_iff_drop_bit_and not_bit_numeral_Bit0_0 numeral_2_eq_2 numeral_Bit0)
+          subgoal for n5 apply (cases n5, simp_all)
+            subgoal for n6 apply (cases n6, simp_all)
+              done
+            done
+          done
+        done
+      done
+    done
+  done
+
+lemma encode_negl_r_4_subgoal_2: " and 15 ((v::u8) >> 4) = 4 \<Longrightarrow> and 15 v \<noteq> 0 \<Longrightarrow>
+    \<not> bit v 3 \<Longrightarrow> \<not> bit v 2 \<Longrightarrow>
+    \<not> bit v (Suc 0)  \<Longrightarrow> bit v 0 \<Longrightarrow> n < 8 \<Longrightarrow> bit (65::u8) n \<Longrightarrow> bit v n"
+  apply (cases n, simp_all)
+  subgoal for n1 apply (cases n1, simp_all)
+    subgoal for n2 apply (cases n2, simp_all)
+      subgoal for n3 apply (cases n3, simp_all)
+        subgoal for n4 apply (cases n4, simp_all)
+          subgoal for n5 apply (cases n5, simp_all)
+            subgoal for n6 apply (cases n6, simp_all)
+              done
+            done
+          done
+        done
+      done
+    done
+  done
+
+
+lemma encode_negl_4_aux : "\<not> bit (v::u8) 3 \<Longrightarrow> \<not> bit v (Suc 0) \<Longrightarrow> \<not> bit (v >> 2) 0 \<Longrightarrow> \<not> bit v 0
+                                   \<Longrightarrow>  and 15 v = 0"
+  apply (rule bit_eqI)
+  apply (simp add: bit_simps)
+  subgoal for n
+  apply (cases n, simp_all)
+  subgoal for n1 apply (cases n1, simp_all)
+    subgoal for n2 apply (cases n2, simp_all)
+      subgoal
+        using numeral_2_eq_2 by argo 
+          subgoal for n3 apply (cases n3, simp_all)
+            using numeral_3_eq_3 by argo
+              done
+            done
+          done
+        done
+
+
+lemma encode_negl_r_4_subgoal_3 : "and 15 ((v::u8) >> 4) = 4 \<Longrightarrow> and 15 v \<noteq> 0 \<Longrightarrow>
+    \<not> bit v 3 \<Longrightarrow> \<not> bit v 2 \<Longrightarrow> \<not> bit v (Suc 0) \<Longrightarrow> \<not> bit v 0 \<Longrightarrow> n < 8 \<Longrightarrow> bit v n \<Longrightarrow> bit (64::u8) n"
+  apply (cases n, simp_all)
+  subgoal for n1 apply (cases n1, simp_all)
+    subgoal for n2 apply (cases n2, simp_all)
+      subgoal
+        by (metis numeral_2_eq_2) 
+      subgoal for n3 apply (cases n3, simp_all)
+        subgoal
+          by (metis numeral_3_eq_3)
+        subgoal for n4 apply (cases n4, simp_all)
+          subgoal
+            by (metis add_2_eq_Suc' bit_1_0 bit_and_iff bit_numeral_Bit1_0 bit_word_iff_drop_bit_and not_bit_numeral_Bit0_0 numeral_2_eq_2 numeral_Bit0)
+          subgoal for n5 apply (cases n5, simp_all)
+            subgoal for n6 apply (cases n6, simp_all)
+              done
+            done
+          done
+        done
+      done
+    done
+  done
+
+
+lemma encode_negl_r_4_subgoal_4: "and 15 ((v::u8) >> 4) = 4 \<Longrightarrow> and 15 v \<noteq> 0 \<Longrightarrow>
+    \<not> bit v 3 \<Longrightarrow> \<not> bit v 2 \<Longrightarrow> \<not> bit v (Suc 0) \<Longrightarrow> \<not> bit v 0 \<Longrightarrow> n < 8 \<Longrightarrow> bit (64::u8) n \<Longrightarrow> bit v n"
+  apply (cases n, simp_all)
+  subgoal for n1 apply (cases n1, simp_all)
+    subgoal for n2 apply (cases n2, simp_all)
+      subgoal for n3 apply (cases n3, simp_all)
+        subgoal for n4 apply (cases n4, simp_all)
+          subgoal for n5 apply (cases n5, simp_all)
+            subgoal for n6 apply (cases n6, simp_all)
+              done
+            done
+          done
+        done
+      done
+    done
+  done
+
+lemma encode_negl_r_1_subgoal_1: " and 7 ((v::u8) >> 3) = 3 \<Longrightarrow> bit v (Suc (Suc (Suc (Suc (Suc 0))))) \<Longrightarrow> False
+ "
+  apply (simp add: bit_eq_iff Suc3_eq_add_3)
+  apply (auto simp add: bit_simps)
+  apply (drule_tac x="2" in spec) by simp
+
+lemma encode_negl_r_4_subgoal_5 : "and 15 ((v::u8) >> 4) = 4 \<Longrightarrow> and 15 v \<noteq> 0 \<Longrightarrow>
+    and 3 ((k::u8) >> 6) = 3 \<Longrightarrow> and 7 (k >> 3) = 3 \<Longrightarrow>
+    \<not> bit v 3 \<Longrightarrow> \<not> bit v 2 \<Longrightarrow> \<not> bit v (Suc 0) \<Longrightarrow> n < 8 \<Longrightarrow> bit k n \<Longrightarrow> \<not> bit (192::u8) n \<Longrightarrow> \<not> bit (24::u8) n \<Longrightarrow> bit (7::u8) n"
+  apply (cases n, simp_all)
+  subgoal for n1 apply (cases n1, simp_all)
+    subgoal for n2 apply (cases n2, simp_all)
+      subgoal for n3 apply (cases n3, simp_all)
+        subgoal for n4 apply (cases n4, simp_all)
+          subgoal for n5 apply (cases n5, simp_all)
+            subgoal
+              using encode_negl_r_1_subgoal_1 by blast
+            subgoal for n6 apply (cases n6, simp_all)
+              done
+            done
+          done
+        done
+      done
+    done
+  done
+
+lemma encode_negl_r_4_subgoal_6: "and 15 ((v::u8) >> 4) = 4 \<Longrightarrow> and 15 v \<noteq> 0 \<Longrightarrow>
+    and 3 ((k::u8) >> 6) = 3 \<Longrightarrow> and 7 (k >> 3) = 3 \<Longrightarrow>
+    \<not> bit v 3 \<Longrightarrow> \<not> bit v 2 \<Longrightarrow> \<not> bit v (Suc 0) \<Longrightarrow> n < 8 \<Longrightarrow> bit k n \<Longrightarrow> \<not> bit (192::u8) n \<Longrightarrow> \<not> bit (24::u8) n \<Longrightarrow> bit (56::u8) n \<Longrightarrow> False"
+  apply (cases n, simp_all)
+  subgoal for n1 apply (cases n1, simp_all)
+    subgoal for n2 apply (cases n2, simp_all)
+      subgoal for n3 apply (cases n3, simp_all)
+        subgoal for n4 apply (cases n4, simp_all)
+          subgoal for n5 apply (cases n5, simp_all)
+            subgoal
+              using encode_negl_r_1_subgoal_1 by blast
+              done
+            done
+          done
+        done
+      done
+    done
+
+lemma encode_negl_r_1_subgoal_2: " and 7 ((v::u8) >> 3) = 3 \<Longrightarrow> bit v (Suc (Suc (Suc (Suc 0)))) "
+  apply (simp add: bit_eq_iff Suc3_eq_add_3 )
+  apply (auto simp add: bit_simps)
+  apply (drule_tac x="1" in spec) by simp
+
+lemma encode_negl_r_4_subgoal_7: "and 15 ((v::u8) >> 4) = 4 \<Longrightarrow> and 15 v \<noteq> 0 \<Longrightarrow>
+    and 3 ((k::u8) >> 6) = 3 \<Longrightarrow> and 7 (k >> 3) = 3 \<Longrightarrow>
+    \<not> bit v 3 \<Longrightarrow> \<not> bit v 2 \<Longrightarrow> \<not> bit v (Suc 0) \<Longrightarrow> n < 8 \<Longrightarrow> \<not> bit (192::u8) n \<Longrightarrow> bit (24::u8) n \<Longrightarrow> bit k n"
+  apply (cases n, simp_all)
+  subgoal for n1 apply (cases n1, simp_all)
+    subgoal for n2 apply (cases n2, simp_all)
+      subgoal for n3 apply (cases n3, simp_all)
+        subgoal
+          by (metis bit_0 bit_and_iff bit_iff_odd_drop_bit bit_numeral_Bit1_0 numeral_3_eq_3)
+        subgoal for n4 apply (cases n4, simp_all)
+          using encode_negl_r_1_subgoal_2 by blast
+              done
+            done
+          done
+        done
+
+lemma encode_negl_r_4_subgoal_8: "and 15 ((v::u8) >> 4) = 4 \<Longrightarrow>  and 15 v \<noteq> 0 \<Longrightarrow>
+    and 3 ((k::u8) >> 6) = 3 \<Longrightarrow> and 7 (k >> 3) = 3 \<Longrightarrow>
+    \<not> bit v 3 \<Longrightarrow> \<not> bit v 2 \<Longrightarrow> \<not> bit v (Suc 0) \<Longrightarrow> n < 8 \<Longrightarrow> 
+    \<not> bit (192::u8) n \<Longrightarrow> bit (7::u8) n \<Longrightarrow> \<not> bit (56::u8) n \<Longrightarrow> bit 8 n \<Longrightarrow> 3 \<le> n \<Longrightarrow> bit v (n - 3) \<Longrightarrow> bit k n"
+  apply (cases n, simp_all)
+  subgoal for n1 apply (cases n1, simp_all)
+    subgoal for n2 apply (cases n2, simp_all)
+      done
+    done
+  done
+
+
+lemma encode_negl_r_4_subgoal_k : "and 15 (v >> 4) = 4 \<Longrightarrow>
+    and 15 v \<noteq> 0 \<Longrightarrow>
+    and 3 (k >> 6) = 3 \<Longrightarrow>
+    and 7 (k >> 3) = 3 \<Longrightarrow>
+    u8_of_ireg dst = or (and 8 (v << 3)) (and 7 k) \<Longrightarrow>
+    \<not> bit v 3 \<Longrightarrow>
+    \<not> bit v 2 \<Longrightarrow>
+    \<not> bit v (Suc 0) \<Longrightarrow>
+    v = or 64 (and (and (and (and (case bit v 0 of True \<Rightarrow> 1 | False \<Rightarrow> 0) (- 3)) (- 5)) (- 9)) (- 241)) \<and>
+    k = or 192 (and (or 24 (and (and 7 (or (and 8 (v << 3)) (and 7 k))) (- 57))) (- 193))"
+  apply (rule conjI)
+  subgoal
+    apply (cases "bit v 0", simp_all)
+    subgoal
+      apply (rule bit_eqI)
+      subgoal for n
+        apply (auto simp add: bit_simps)
+        subgoal using encode_negl_r_4_subgoal_1 by simp
+        subgoal using encode_negl_r_4_subgoal_2 by simp
+        done
+      done
+
+    subgoal
+      apply (rule bit_eqI)
+      subgoal for n
+        apply (auto simp add: bit_simps)
+        subgoal using encode_negl_r_4_subgoal_3 by simp
+        subgoal using encode_negl_r_4_subgoal_4 by simp
+        done                          
+      done
+    done
+
+    subgoal
+      apply (rule bit_eqI)
+      subgoal for n
+        apply (auto simp add: bit_simps)
+        subgoal using encode_negl_r_4_subgoal_5 by simp
+        subgoal using encode_negl_r_4_subgoal_5 by simp
+        subgoal using encode_negl_r_4_subgoal_5 by simp
+        subgoal using encode_negl_r_4_subgoal_6 by simp
+        subgoal using encode_negl_r_4_subgoal_7 by simp
+        subgoal using encode_negl_r_4_subgoal_8 by simp
+        done
+      done
+    done
+
+lemma encode_negl_r_4: "
+    and 15 (v >> 4) = 4 \<Longrightarrow> and 15 v \<noteq> 0 \<Longrightarrow> and 3 (k >> 6) = 3 \<Longrightarrow> and 7 (k >> 3) = 3 \<Longrightarrow>      
+    ireg_of_u8 (bitfield_insert_u8 3 (Suc 0) (and 7 k) (and 1 v)) = Some dst \<Longrightarrow>
+    \<not> bit v 3 \<Longrightarrow> \<not> bit v 2 \<Longrightarrow> \<not> bit v (Suc 0) \<Longrightarrow>
+    bitfield_insert_u8 4 4
+     (bitfield_insert_u8 3 (Suc 0)
+       (bitfield_insert_u8 2 (Suc 0) (bitfield_insert_u8 (Suc 0) (Suc 0) (u8_of_bool (and (u8_of_ireg dst) 8 \<noteq> 0)) 0) 0) 0)
+     4 \<noteq> 64 \<Longrightarrow>
+    v =
+    bitfield_insert_u8 4 4
+     (bitfield_insert_u8 3 (Suc 0)
+       (bitfield_insert_u8 2 (Suc 0) (bitfield_insert_u8 (Suc 0) (Suc 0) (u8_of_bool (and (u8_of_ireg dst) 8 \<noteq> 0)) 0) 0) 0)
+     4 \<and>
+    k = bitfield_insert_u8 6 2 (bitfield_insert_u8 3 3 (and 7 (u8_of_ireg dst)) 3) 3"
+  apply (simp add: u8_of_ireg_of_u8_iff[symmetric])
+  apply (unfold bitfield_insert_u8_def u8_of_bool_def Let_def)
+  apply simp
+  using encode_negl_r_4_subgoal_k by simp
+
+end
