theory/x64_encode_negq_r_1.thy
@@ -1,0 +1,75 @@
+theory x64_encode_negq_r_1
+imports
+  Main
+  rBPFCommType
+  x64Syntax BitsOpMore
+begin
+
+lemma encode_negq_r_1_subgoal_1: 
+" and 15 (v >> 4) = 4 \<Longrightarrow> and 15 v \<noteq> 0 \<Longrightarrow> and 3 (k >> 6) = 3 \<Longrightarrow> and 7 (k >> 3) = 3 \<Longrightarrow>
+  bit v 3 \<Longrightarrow> \<not> bit v 2 \<Longrightarrow>\<not> bit v (Suc 0) \<Longrightarrow> bit v 0 \<Longrightarrow>
+  bit k 0 = bit (or 192 (and (or 24 (and (and 7 (or (and 8 (v << 3)) (and 7 k))) (- 57))) (- 193))) 0"
+
+
+
+lemma encode_negq_r_1_subgoal_k: " and 15 (v >> 4) = 4 \<Longrightarrow> and 15 v \<noteq> 0 \<Longrightarrow>
+    and 3 (k >> 6) = 3 \<Longrightarrow> and 7 (k >> 3) = 3 \<Longrightarrow>
+    u8_of_ireg dst = or (and 8 (v << 3)) (and 7 k) \<Longrightarrow>
+    bit v 3 \<Longrightarrow> \<not> bit v 2 \<Longrightarrow> \<not> bit v (Suc 0) \<Longrightarrow> bit v 0 \<Longrightarrow> 
+    v = 73 \<and> k = or 192 (and (or 24 (and (and 7 (or (and 8 (v << 3)) (and 7 k))) (- 57))) (- 193))"
+  apply (rule conjI)
+   apply (rule bit_eqI)
+
+  subgoal for n1 apply (cases n1, simp_all)
+    subgoal for n2 apply (cases n2, simp_all)
+      subgoal for n3 apply (cases n3, simp_all)
+        subgoal
+          using numeral_2_eq_2 by argo
+        subgoal for n4 apply (cases n4, simp_all)
+          subgoal
+            using numeral_3_eq_3 by argo
+          subgoal for n5 apply (cases n5, simp_all)
+            subgoal
+              by (metis add_2_eq_Suc' bit_1_0 bit_and_iff bit_numeral_Bit1_0 bit_word_iff_drop_bit_and not_bit_numeral_Bit0_0 numeral_2_eq_2 numeral_Bit0) 
+            subgoal for n6 apply (cases n6, simp_all)
+              subgoal for n7 apply (cases n7, simp_all)
+              done
+            done
+          done
+        done
+      done
+    done
+  done
+
+  apply (rule bit_eqI)
+  subgoal for n1 apply (cases n1, simp_all)
+    subgoal
+
+
+
+
+
+
+lemma encode_negq_r_1: "
+    and 15 (v >> 4) = 4 \<Longrightarrow> and 15 v \<noteq> 0 \<Longrightarrow>
+    and 3 (k >> 6) = 3 \<Longrightarrow> and 7 (k >> 3) = 3 \<Longrightarrow>
+    ireg_of_u8 (bitfield_insert_u8 3 (Suc 0) (and 7 k) (and 1 v)) = Some dst \<Longrightarrow>
+    bit v 3 \<Longrightarrow> \<not> bit v 2 \<Longrightarrow> \<not> bit v (Suc 0) \<Longrightarrow>
+    v =
+    bitfield_insert_u8 4 4
+     (bitfield_insert_u8 3 (Suc 0) (bitfield_insert_u8 2 (Suc 0) (bitfield_insert_u8 (Suc 0) (Suc 0) (u8_of_bool (and (u8_of_ireg dst) 8 \<noteq> 0)) 0) 0) 1)
+     4 \<and>
+    k = bitfield_insert_u8 6 2 (bitfield_insert_u8 3 3 (and 7 (u8_of_ireg dst)) 3) 3
+"
+
+  apply (simp add: u8_of_ireg_of_u8_iff[symmetric])
+  apply (unfold bitfield_insert_u8_def u8_of_bool_def Let_def)
+  apply simp
+  subgoal
+    apply (cases "bit v 0", simp_all)
+    subgoal
+      using 
+  done
+
+end
+
